lib_list/ArrayListGen.fsti
@@ -113,7 +113,7 @@ val intro_arraylist_nil (#a:Type) (#opened:inames)
     )
 
 /// If the head of one of the lists is not null, then it is in the list
-val intro_head1_not_null_mem (#a:Type) (#opened:inames)
+val lemma_head1_not_null_mem (#a:Type) (#opened:inames)
   (pred1 pred2 pred3: a -> prop)
   (r:A.array (cell a))
   (hd1 hd2 hd3:US.t) :
@@ -127,6 +127,42 @@ val intro_head1_not_null_mem (#a:Type) (#opened:inames)
       h1 (varraylist pred1 pred2 pred3 r (US.v hd1) (US.v hd2) (US.v hd3)) /\
       // Functional property
       mem (US.v hd1) (US.v hd1) (h1 (varraylist pred1 pred2 pred3 r (US.v hd1) (US.v hd2) (US.v hd3)))
+    )
+
+/// If the head of one of the lists is not null, then it is smaller than the length
+/// of the underlying array
+val lemma_head1_in_bounds (#a:Type) (#opened:inames)
+  (pred1 pred2 pred3: a -> prop)
+  (r:A.array (cell a))
+  (hd1 hd2 hd3:US.t) :
+  SteelGhost unit opened
+    (varraylist pred1 pred2 pred3 r (US.v hd1) (US.v hd2) (US.v hd3))
+    (fun _ -> varraylist pred1 pred2 pred3 r (US.v hd1) (US.v hd2) (US.v hd3))
+    (requires fun _ -> hd1 <> null_ptr)
+    (ensures fun h0 _ h1 ->
+      // Framing
+      h0 (varraylist pred1 pred2 pred3 r (US.v hd1) (US.v hd2) (US.v hd3)) ==
+      h1 (varraylist pred1 pred2 pred3 r (US.v hd1) (US.v hd2) (US.v hd3)) /\
+      // Functional property
+      US.v hd1 < A.length r
+    )
+
+/// If the head of one of the lists is not null, then it satisfies the corresponding predicate
+val lemma_head1_implies_pred1 (#a:Type) (#opened:inames)
+  (pred1 pred2 pred3: a -> prop)
+  (r:A.array (cell a))
+  (hd1:US.t{US.v hd1 < A.length r})
+  (hd2 hd3:US.t) :
+  SteelGhost unit opened
+    (varraylist pred1 pred2 pred3 r (US.v hd1) (US.v hd2) (US.v hd3))
+    (fun _ -> varraylist pred1 pred2 pred3 r (US.v hd1) (US.v hd2) (US.v hd3))
+    (requires fun h -> hd1 <> null_ptr)
+    (ensures fun h0 _ h1 ->
+      // Framing
+      h0 (varraylist pred1 pred2 pred3 r (US.v hd1) (US.v hd2) (US.v hd3)) ==
+      h1 (varraylist pred1 pred2 pred3 r (US.v hd1) (US.v hd2) (US.v hd3)) /\
+      // Functional property
+      pred1 (get_data (Seq.index (h1 (varraylist pred1 pred2 pred3 r (US.v hd1) (US.v hd2) (US.v hd3))) (US.v hd1)))
     )
 
 /// Reads at index [idx] in the array.
